# $\color{aqua}{基本命题：1}$
> + ## $若\psi_1和\psi_2是定态薛定谔方程的两个解则它们的朗斯基行列式为\textcolor{red}{常数}$
_Proof:_
>$$
-\frac{\hbar^2}{2m}\frac{d^2}{dx^2}\psi_1+V\psi_1=E\psi_1 \qquad \textcircled{1}
$$
$$
-\frac{\hbar^2}{2m}\frac{d^2}{dx^2}\psi_2+V\psi_2=E\psi_2 \qquad \textcircled{2}
$$
$\textcircled{1}\times\psi_2 - \textcircled{2}\times\psi_1:$
$$
-\frac{\hbar^2}{2m}\frac{d^2}{dx^2}\psi_1\psi_2+V\psi_1\psi_2+\frac{\hbar^2}{2m}\frac{d^2}{dx^2}\psi_1\psi_2-V\psi_2\psi_1=E\psi_1\psi_2-E\psi_2\psi_1 \\
-\frac{\hbar^2}{2m}\psi_1^{''}\psi_2+\frac{\hbar^2}{\psi_2}^{''}\psi_1=0\\
-\frac{\hbar^2}{2m}(\psi_1^{''}\psi_2-\psi_1^{''}\psi_2)=0\\
\psi_2^{''}\psi_1-\psi_1^{''}\psi_1=0\\
\psi_2^{""}\psi_1+\psi_2^{'}\psi_1^{'}-\psi_2^{'}\psi_1^{'}-\psi_1^{''}\psi_2=0\\
\psi_2^{''}\psi_1+\psi_2^{'}\psi_1^{'}-(\psi_2^{'}\psi_1^{'}+\psi_1^{''}\psi_2)=0\\
(\psi_2^{'}\psi_1)^{'}-(\psi_1^{'}\psi_2)^{'}=0\\
[(\psi_2^{'}\psi_1)-(\psi_1^{'}\psi_2)]^{'}=0\\
故\psi_2^{'}\psi_1-\psi_1^{'}\psi_2=\textcolor{red}{C}\\
Q.E.D
$$